theories/SLFExtra.v
@@ -4,8 +4,10 @@ Separation Logic Foundations
 
 Chapter: "Extra".
 
-This file provides formalization of reasoning rules expressed
-using Separation Logic triples.
+This file provides formalization of additional reasoning rules 
+expressed using Separation Logic triples. 
+
+This file serves as a reference, there is no need to read through it.
 
 Author: Arthur Charguéraud.
 License: MIT.
